pcuic/theories/PCUICArities.v
@@ -1,0 +1,558 @@
+(* Distributed under the terms of the MIT license.   *)
+
+From Coq Require Import Bool String List Program BinPos Compare_dec Arith Lia
+     Classes.CRelationClasses ProofIrrelevance.
+From MetaCoq.Template Require Import config Universes monad_utils utils BasicAst
+     AstUtils UnivSubst.
+From MetaCoq.PCUIC Require Import PCUICAst PCUICAstUtils PCUICInduction
+     PCUICReflect PCUICLiftSubst PCUICUnivSubst PCUICTyping
+     PCUICCumulativity PCUICSR PCUICPosition PCUICEquality PCUICNameless
+     PCUICAlpha PCUICNormal PCUICInversion PCUICCumulativity PCUICReduction
+     PCUICConfluence PCUICConversion PCUICContextConversion PCUICValidity
+     PCUICParallelReductionConfluence PCUICWeakeningEnv
+     PCUICClosed PCUICPrincipality PCUICSubstitution
+     PCUICWeakening PCUICGeneration PCUICUtils PCUICContexts.
+From Equations Require Import Equations.
+
+Require Import Equations.Prop.DepElim.
+Require Import Equations.Type.Relation_Properties.
+
+Lemma isArity_it_mkProd_or_LetIn Γ t : isArity t -> isArity (it_mkProd_or_LetIn Γ t).
+Proof.
+  intros isA. induction Γ using rev_ind; simpl; auto.
+  rewrite it_mkProd_or_LetIn_app. simpl; auto.
+  destruct x as [? [?|] ?]; simpl; auto.
+Qed.
+
+Lemma invert_cumul_arity_l {cf:checker_flags} Σ (Γ : context) (C : term) T :
+  wf Σ.1 ->
+  Σ;;; Γ |- C <= T ->
+  match destArity [] C with
+  | Some (ctx, s) =>
+    ∑ T' ctx' s', red Σ.1 Γ T T' * (destArity [] T' = Some (ctx', s')) * 
+       conv_context Σ (Γ ,,, smash_context [] ctx) (Γ ,,, ctx') * leq_universe
+       (global_ext_constraints Σ) s s'
+  | None => unit
+  end.
+Proof.
+intros wfΣ CT.
+generalize (destArity_spec [] C). destruct destArity as [[ctx p]|].
+simpl. intros ->. 2:intros _; exact tt.
+revert Γ T CT.
+generalize (@le_n #|ctx|).
+generalize (#|ctx|) at 2. intros n; revert ctx.
+induction n; intros ctx Hlen Γ T HT.
+- destruct ctx; simpl in Hlen; try lia.
+  eapply invert_cumul_sort_l in HT as [u' [redT leqT]].
+  exists (tSort u'), [], u'; intuition auto.
+  reflexivity.
+- destruct ctx using rev_ind.
+  * eapply invert_cumul_sort_l in HT as [u' [redT leqT]].
+    exists (tSort u'), [], u'; intuition auto.  
+    reflexivity.
+  * rewrite it_mkProd_or_LetIn_app in HT; simpl in HT.
+    destruct x as [na [b|] ty]; unfold mkProd_or_LetIn in HT; simpl in *.
+    + eapply invert_cumul_letin_l in HT; auto.
+      unfold subst1 in HT; rewrite subst_it_mkProd_or_LetIn in HT.
+      rewrite app_length /= Nat.add_1_r in Hlen.
+      simpl in HT. specialize (IHn (subst_context [b] 0 ctx) ltac:(rewrite
+      subst_context_length; lia) Γ T HT).
+      destruct IHn as [T' [ctx' [s' [[[redT destT] convctx] leq]]]].
+      clear IHctx.
+      exists T', ctx', s'. intuition auto.
+      rewrite smash_context_app. simpl.
+      now rewrite -smash_context_subst_empty.
+    + eapply invert_cumul_prod_l in HT; auto. 
+      rewrite -> app_length in Hlen.
+      rewrite Nat.add_1_r in Hlen.
+      destruct HT as [na' [A' [B' [[redT convT] HT]]]].
+      specialize (IHn ctx ltac:(lia) (Γ ,, vass na ty) B' HT). clear IHctx.
+      destruct IHn as [T' [ctx' [s' [[[redT' destT] convctx] leq]]]].
+      exists (tProd na' A' T'), (ctx' ++ [vass na' A'])%list, s'. intuition auto. 2:simpl.
+      -- transitivity (tProd na' A' B'); auto.
+        eapply red_prod. reflexivity.
+        todo"red context conv"%string.
+      -- now rewrite destArity_app destT.
+      -- rewrite smash_context_app /= .
+         rewrite !app_context_assoc. simpl.
+         eapply conv_context_trans with (Γ ,, vass na ty ,,, ctx'); auto.
+         todo "conv context"%string.
+Qed.
+
+
+Lemma destArity_spec_Some ctx T ctx' s :
+  destArity ctx T = Some (ctx', s)
+  -> it_mkProd_or_LetIn ctx T = it_mkProd_or_LetIn ctx' (tSort s).
+Proof.
+  pose proof (PCUICClosed.destArity_spec ctx T) as H.
+  intro e; now rewrite e in H.
+Qed.
+
+Lemma isWAT_tProd {cf:checker_flags} {Σ : global_env_ext} (HΣ' : wf Σ)
+      {Γ} (HΓ : wf_local Σ Γ) {na A B}
+  : isWfArity_or_Type Σ Γ (tProd na A B)
+    <~> (isType Σ Γ A × isWfArity_or_Type Σ (Γ,, vass na A) B).
+Proof.
+  split; intro HH.
+  - destruct HH as [[ctx [s [H1 H2]]]|[s H]].
+    + cbn in H1. apply destArity_app_Some in H1.
+      destruct H1 as [ctx' [H1 HH]]; subst ctx.
+      rewrite app_context_assoc in H2. split.
+      * apply wf_local_app in H2. inversion H2; subst. assumption.
+      * left. exists ctx', s. split; tas.
+    + apply inversion_Prod in H; tas. destruct H as [s1 [s2 [HA [HB Hs]]]].
+      split.
+      * eexists; tea.
+      * right. eexists; tea.
+  - destruct HH as [HA [[ctx [s [H1 H2]]]|HB]].
+    + left. exists ([vass na A] ,,, ctx), s. split.
+      cbn. now rewrite destArity_app H1.
+      now rewrite app_context_assoc.
+    + right. destruct HA as [sA HA], HB as [sB HB].
+      eexists. econstructor; eassumption.
+Defined.
+
+Lemma isWAT_subst {cf:checker_flags} {Σ : global_env_ext} (HΣ' : wf Σ)
+      {Γ Δ} (HΓ : wf_local Σ (Γ ,,, Δ)) {A} s :
+    subslet Σ Γ s Δ ->
+    isWfArity_or_Type Σ (Γ ,,, Δ) A -> 
+    isWfArity_or_Type Σ Γ (subst0 s A).
+Proof.
+  intros sub WAT.
+  destruct WAT.
+  - left.
+    destruct i as [ctx [s' [wfa wfl]]].
+    exists (subst_context s 0 ctx), s'.
+    generalize (subst_destArity [] A s 0).
+    rewrite wfa. simpl. intros ->.
+    split; auto.
+    now eapply substitution_wf_local.
+  - right.
+    destruct i as [s' Hs].
+    exists s'. eapply (substitution _ _ Δ s [] _ _ HΣ' sub Hs).
+    now apply wf_local_app in HΓ.
+Qed.
+
+Lemma isWAT_tLetIn {cf:checker_flags} {Σ : global_env_ext} (HΣ' : wf Σ)
+      {Γ} (HΓ : wf_local Σ Γ) {na t A B}
+  : isWfArity_or_Type Σ Γ (tLetIn na t A B)
+    <~> (isType Σ Γ A × (Σ ;;; Γ |- t : A)
+                      × isWfArity_or_Type Σ (Γ,, vdef na t A) B).
+Proof.
+  split; intro HH.
+  - destruct HH as [[ctx [s [H1 H2]]]|[s H]].
+    + cbn in H1. apply destArity_app_Some in H1.
+      destruct H1 as [ctx' [H1 HH]]; subst ctx.
+      rewrite app_context_assoc in H2. repeat split.
+      * apply wf_local_app in H2. inversion H2; subst. assumption.
+      * apply wf_local_app in H2. inversion H2; subst. assumption.
+      * left. exists ctx', s. split; tas.
+    + apply inversion_LetIn in H; tas. destruct H as [s1 [A' [HA [Ht [HB H]]]]].
+      repeat split; tas. 1: eexists; eassumption.
+      apply cumul_Sort_r_inv in H.
+      destruct H as [s' [H H']].
+      right. exists s'. eapply type_reduction; tea.
+      1:{ constructor; tas. eexists; tea. }
+      apply invert_red_letin in H; tas.
+      destruct H as [[? [? [? [? [[[H ?] ?] ?]]]]]|H].
+      * apply invert_red_sort in H; inv H.
+      * etransitivity.
+        2: apply weakening_red_0 with (Γ' := [_]) (N := tSort _);
+          tea; reflexivity.
+        exact (red_rel_all _ (Γ ,, vdef na t A) 0 t A' eq_refl).
+  - destruct HH as [HA [Ht [[ctx [s [H1 H2]]]|HB]]].
+    + left. exists ([vdef na t A] ,,, ctx), s. split.
+      cbn. now rewrite destArity_app H1.
+      now rewrite app_context_assoc.
+    + right. destruct HB as [sB HB].
+      eexists. eapply type_reduction; tas.
+      * econstructor; tea.
+        apply HA.π2.
+      * apply red1_red.
+        apply red_zeta with (b':=tSort sB).
+Defined.
+
+
+
+Lemma typing_spine_strengthen {cf:checker_flags} Σ Γ T T' args U : 
+  wf Σ.1 ->
+  typing_spine Σ Γ T args U ->
+  isWfArity_or_Type Σ Γ T' ->
+  Σ ;;; Γ |- T' <= T ->
+  ∑ U', (typing_spine Σ Γ T' args U') * (Σ ;;; Γ |- U' <= U).
+Proof.
+  induction 2 in T' |- *; intros WAT redT.
+  - exists T'.
+    split. constructor. auto. reflexivity. transitivity ty; auto.
+  - eapply invert_cumul_prod_r in c as [na' [A' [B'' HT]]]; auto.
+    destruct HT as [[redT' convA] cumulB].
+    assert (Σ ;;; Γ |- T' <= tProd na' A' B'').
+    transitivity T; auto. now eapply red_cumul.
+    eapply invert_cumul_prod_r in X1 as [na'' [A'' [B''' [[redt' convA'] cumulB''']]]]; auto.
+    specialize (IHX0 (B''' {0 := hd})).
+    have WAT' : isWfArity_or_Type Σ Γ (tProd na'' A'' B'''). {
+      eapply (isWfArity_or_Type_red (A:=T')); auto.
+    }
+    have WAT'': isWfArity_or_Type Σ Γ (B''' {0 := hd}). 
+    { eapply isWAT_tProd in WAT' as [AWAT BWAT].
+      eapply (isWAT_subst(Δ := [vass na'' A'']) X); eauto.
+      constructor; eauto using typing_wf_local.
+      constructor. constructor. rewrite subst_empty.
+      eapply type_Cumul; eauto. transitivity A'; auto using conv_alt_cumul.
+      auto. eauto using typing_wf_local. }
+    forward IHX0 by auto.
+    forward IHX0. {
+      transitivity (B'' {0 := hd}); auto.
+      eapply substitution_cumul0; eauto.
+      eapply substitution_cumul0; eauto.            
+    }
+    destruct IHX0 as [U' [spineU' leU']].
+    exists U'; split.
+    eapply type_spine_cons with na'' A'' B'''; auto.
+    now eapply red_cumul. 
+    eapply type_Cumul with A; eauto.
+    eapply isWAT_tProd in WAT'; intuition eauto using typing_wf_local.
+    transitivity A'; auto using conv_alt_cumul.
+    assumption.
+Qed.
+
+
+Lemma arity_typing_spine {cf:checker_flags} Σ Γ Γ' s inst s' : 
+  wf Σ.1 ->
+  wf_local Σ Γ ->
+  wf_local Σ (Γ ,,, Γ') ->
+  typing_spine Σ Γ (it_mkProd_or_LetIn Γ' (tSort s)) inst (tSort s') ->
+  #|inst| = context_assumptions Γ' /\ leq_universe (global_ext_constraints Σ) s s'.
+Proof.
+  intros wfΣ wfΓ wfΓ'; revert s inst s'.
+  generalize (le_n #|Γ'|).
+  generalize (#|Γ'|) at 2.
+  induction n in Γ', wfΓ' |- *. 
+  destruct Γ' using rev_ind; try clear IHΓ'; simpl; intros len s inst s' Hsp.
+  - depelim Hsp. intuition auto.
+    now eapply cumul_Sort_inv.
+    now eapply cumul_Sort_Prod_inv in c.
+  - rewrite app_length /= in len; elimtype False; lia.
+  - intros len s inst s' Hsp.
+    destruct Γ' using rev_ind; try clear IHΓ'.
+    -- depelim Hsp. intuition auto.
+      now eapply cumul_Sort_inv.
+      now eapply cumul_Sort_Prod_inv in c.
+    -- rewrite app_length /= in len.
+      rewrite it_mkProd_or_LetIn_app in Hsp.
+      destruct x as [na [b|] ty]; simpl in *; rewrite /mkProd_or_LetIn /= in Hsp.
+      + rewrite context_assumptions_app /= Nat.add_0_r.
+        eapply typing_spine_letin_inv in Hsp; auto.
+        rewrite /subst1 subst_it_mkProd_or_LetIn /= in Hsp.
+        specialize (IHn (subst_context [b] 0 l)).
+        forward IHn. {
+          rewrite app_context_assoc in wfΓ'.
+          apply All_local_env_app in wfΓ' as [wfb wfa].
+          depelim wfb. simpl in H; noconf H. simpl in H. noconf H.
+          eapply substitution_wf_local. eauto. 
+          epose proof (cons_let_def Σ Γ [] [] na b ty ltac:(constructor)).
+          rewrite !subst_empty in X. eapply X. auto.
+          eapply All_local_env_app_inv; split.
+          constructor; auto. apply wfa. }
+        forward IHn by rewrite subst_context_length; lia.
+        specialize (IHn s inst s'). 
+        now rewrite context_assumptions_subst in IHn.
+      + rewrite context_assumptions_app /=.
+        depelim Hsp. 
+        now eapply cumul_Prod_Sort_inv in c.
+        eapply cumul_Prod_inv in c as [conva cumulB].
+        eapply (substitution_cumul0 _ _ _ _ _ _ hd) in cumulB; auto.
+        rewrite /subst1 subst_it_mkProd_or_LetIn /= in cumulB.
+        specialize (IHn (subst_context [hd] 0 l)).
+        forward IHn. {
+          rewrite app_context_assoc in wfΓ'.
+          apply All_local_env_app in wfΓ' as [wfb wfa]; eauto.
+          depelim wfb. simpl in H; noconf H.
+          eapply substitution_wf_local. auto. 
+          constructor. constructor. rewrite subst_empty.
+          eapply type_Cumul. eapply t.
+          right; eapply l0.
+          eapply conv_alt_cumul; auto. now symmetry. 
+          eapply All_local_env_app_inv; eauto; split.
+          constructor; eauto. eapply isWAT_tProd in i; intuition eauto.
+          simpl in H; noconf H.
+        }
+        forward IHn by rewrite subst_context_length; lia.
+        specialize (IHn s tl s'). 
+        rewrite context_assumptions_subst in IHn.
+        eapply typing_spine_strengthen in Hsp.
+        4:eapply cumulB. all:eauto.
+        simpl. destruct Hsp as [U' [sp' cum]].
+        eapply typing_spine_weaken_concl in sp'; eauto using cum.
+        intuition auto. now rewrite H0; lia.
+        left; eexists _, _; intuition auto.
+        left; eexists (subst_context [hd] 0 l), s; intuition auto.
+        now rewrite destArity_it_mkProd_or_LetIn /= app_context_nil_l.
+        eapply substitution_wf_local; eauto. constructor. constructor.
+        rewrite subst_empty. eapply type_Cumul. eapply t.
+        2:{ eapply conv_alt_cumul. auto. symmetry. eassumption. } 
+        eapply All_local_env_app in wfΓ' as [wfb wfa].
+        eapply All_local_env_app in wfa as [wfa' wfa''].
+        depelim wfa'. simpl in H; noconf H. right; auto.
+        simpl in H; noconf H. 
+        unfold snoc. rewrite app_context_assoc in wfΓ'. eapply wfΓ'.
+Qed.
+
+Lemma mkApps_ind_typing_spine {cf:checker_flags} Σ Γ Γ' ind i
+  inst ind' i' args args' : 
+  wf Σ.1 ->
+  wf_local Σ Γ ->
+  isWfArity_or_Type Σ Γ (it_mkProd_or_LetIn Γ' (mkApps (tInd ind i) args)) ->
+  typing_spine Σ Γ (it_mkProd_or_LetIn Γ' (mkApps (tInd ind i) args)) inst 
+    (mkApps (tInd ind' i') args') ->
+  #|inst| = context_assumptions Γ' /\ ind = ind'.
+Proof.
+  intros wfΣ wfΓ; revert args args' ind i ind' i' inst.
+  generalize (le_n #|Γ'|).
+  generalize (#|Γ'|) at 2.
+  induction n in Γ' |- *. 
+  destruct Γ' using rev_ind; try clear IHΓ'; simpl; intros len args args' ind i ind' i' inst wat Hsp.
+  - depelim Hsp. intuition auto.
+    eapply invert_cumul_ind_l in c as [? [? [? ?]]]; auto.
+    eapply invert_red_ind in r as [? [eq ?]]. now solve_discr.
+    eapply invert_cumul_prod_r in c as [? [? [? [[? ?] ?]]]]; auto.
+    eapply invert_red_ind in r as [? [eq ?]]. now solve_discr.
+  - rewrite app_length /= in len; elimtype False; lia.
+  - intros len args args' ind i ind' i' inst wat Hsp.
+    destruct Γ' using rev_ind; try clear IHΓ'.
+    -- depelim Hsp. intuition auto.
+      eapply invert_cumul_ind_l in c as [? [? [? ?]]]; auto.
+      eapply invert_red_ind in r as [? [eq ?]]. now solve_discr.
+      eapply invert_cumul_prod_r in c as [? [? [? [[? ?] ?]]]]; auto.
+      eapply invert_red_ind in r as [? [eq ?]]. now solve_discr.
+    -- rewrite app_length /= in len.
+      rewrite it_mkProd_or_LetIn_app in Hsp.
+      destruct x as [na [b|] ty]; simpl in *; rewrite /mkProd_or_LetIn /= in Hsp.
+      + rewrite context_assumptions_app /= Nat.add_0_r.
+        eapply typing_spine_letin_inv in Hsp; auto.
+        rewrite /subst1 subst_it_mkProd_or_LetIn /= in Hsp.
+        specialize (IHn (subst_context [b] 0 l)).
+        forward IHn by rewrite subst_context_length; lia.
+        rewrite subst_mkApps Nat.add_0_r in Hsp.
+        specialize (IHn (map (subst [b] #|l|) args) args' ind i ind' i' inst).
+        forward IHn. {
+          move: wat; rewrite it_mkProd_or_LetIn_app /= /mkProd_or_LetIn /= => wat.
+          eapply isWfArity_or_Type_red in wat; last first. eapply red1_red.
+          constructor. auto.
+          now rewrite /subst1 subst_it_mkProd_or_LetIn subst_mkApps Nat.add_0_r
+          in wat. }
+        now rewrite context_assumptions_subst in IHn.
+      + rewrite context_assumptions_app /=.
+        pose proof (typing_spine_WAT_concl Hsp).
+        depelim Hsp.
+        eapply invert_cumul_prod_l in c as [? [? [? [[? ?] ?]]]]; auto.
+        eapply invert_red_ind in r as [? [eq ?]]. now solve_discr.
+        eapply cumul_Prod_inv in c as [conva cumulB].
+        eapply (substitution_cumul0 _ _ _ _ _ _ hd) in cumulB; auto.
+        rewrite /subst1 subst_it_mkProd_or_LetIn /= in cumulB.
+        specialize (IHn (subst_context [hd] 0 l)).
+        forward IHn by rewrite subst_context_length; lia.
+        specialize (IHn (map (subst [hd] #|l|) args) args' ind i ind' i' tl). all:auto.
+        have isWATs: isWfArity_or_Type Σ Γ
+        (it_mkProd_or_LetIn (subst_context [hd] 0 l)
+           (mkApps (tInd ind i) (map (subst [hd] #|l|) args))). {
+          move: wat; rewrite it_mkProd_or_LetIn_app /= /mkProd_or_LetIn /= => wat.
+          eapply isWAT_tProd in wat; auto. destruct wat as [isty wat].
+          epose proof (isWAT_subst wfΣ (Γ:=Γ) (Δ:=[vass na ty])).
+          forward X0. constructor; auto.
+          specialize (X0 (it_mkProd_or_LetIn l (mkApps (tInd ind i) args)) [hd]).
+          forward X0. constructor. constructor. rewrite subst_empty; auto.
+          eapply isWAT_tProd in i0; auto. destruct i0. 
+          eapply type_Cumul with A; auto. now eapply conv_alt_cumul.
+          now rewrite /subst1 subst_it_mkProd_or_LetIn subst_mkApps Nat.add_0_r
+          in X0. }
+        rewrite subst_mkApps Nat.add_0_r in cumulB. simpl in *. 
+        rewrite context_assumptions_subst in IHn.
+        eapply typing_spine_strengthen in Hsp.
+        4:eapply cumulB. all:eauto.
+        simpl. destruct Hsp as [U' [sp' cum]].
+        eapply typing_spine_weaken_concl in sp'; eauto using cum.
+        intuition auto. now rewrite H; lia.
+Qed.
+
+
+Lemma type_it_mkProd_or_LetIn {cf:checker_flags} Σ Γ Γ' u t s : 
+  wf Σ.1 ->
+  type_local_ctx (lift_typing typing) Σ Γ Γ' u ->
+  Σ ;;; Γ ,,, Γ' |- t : tSort s ->
+  Σ ;;; Γ |- it_mkProd_or_LetIn Γ' t : tSort (Universe.sort_of_product u s).
+Proof.
+  revert Γ u s t.
+  induction Γ'; simpl; auto; move=> Γ u s t wfΣ equ Ht.
+  - eapply type_Cumul; eauto.
+    left. eexists [], _; intuition eauto.
+    eapply typing_wf_local; eauto.
+    constructor. constructor.
+    eapply leq_universe_product.
+  - specialize (IHΓ' Γ  u (Universe.sort_of_product u s)); auto.
+    unfold app_context in Ht.
+    eapply type_Cumul.
+    eapply IHΓ'; auto.
+    destruct a as [na [b|] ty]; intuition auto.
+    destruct a as [na [b|] ty]; intuition auto.
+    { apply typing_wf_local in Ht as XX. inversion XX; subst.
+      eapply (type_mkProd_or_LetIn _ _ {| decl_body := Some b |}); auto.
+      + simpl. exact X0.π2.
+      + eapply type_Cumul; eauto.
+        left. eexists [], _. intuition eauto.
+        constructor. constructor. eapply leq_universe_product. }
+    eapply (type_mkProd_or_LetIn _ _ {| decl_body := None |}) => /=; eauto.
+    left. eexists [], _; intuition eauto using typing_wf_local.
+    eapply typing_wf_local in Ht.
+    depelim Ht; eapply All_local_env_app in Ht; intuition auto.
+    constructor. constructor.
+    apply eq_universe_leq_universe.
+    apply sort_of_product_twice.
+Qed.
+
+Local Open Scope string_scope.
+
+Lemma typing_spine_weaken_concl {cf:checker_flags} {Σ Γ T args S S'} : 
+  wf Σ.1 ->
+  typing_spine Σ Γ T args S ->
+  Σ ;;; Γ |- S <= S' ->
+  isWfArity_or_Type Σ Γ S' ->
+  typing_spine Σ Γ T args S'.
+Proof.
+  intros wfΣ.  
+  induction 1 in S' => cum.
+  constructor; auto. now transitivity ty'.
+  intros isWAT.
+  econstructor; eauto.
+Qed.
+
+Lemma typing_spine_letin_inv {cf:checker_flags} {Σ Γ na b B T args S} : 
+  wf Σ.1 ->
+  typing_spine Σ Γ (tLetIn na b B T) args S ->
+  typing_spine Σ Γ (T {0 := b}) args S.
+Proof.
+  intros wfΣ Hsp.
+  depelim Hsp.
+  constructor. auto.
+  now eapply invert_cumul_letin_l in c.
+  econstructor; eauto.
+  now eapply invert_cumul_letin_l in c.
+Qed.
+
+Lemma typing_spine_letin {cf:checker_flags} {Σ Γ na b B T args S} : 
+  wf Σ.1 ->
+  typing_spine Σ Γ (T {0 := b}) args S ->
+  typing_spine Σ Γ (tLetIn na b B T) args S.
+Proof.
+  intros wfΣ Hsp.
+  depelim Hsp.
+  constructor. auto.
+  etransitivity. eapply red_cumul. eapply red1_red, red_zeta. auto.
+  econstructor; eauto.
+  etransitivity. eapply red_cumul. eapply red1_red, red_zeta. auto.
+Qed.
+
+Lemma typing_spine_prod {cf:checker_flags} {Σ Γ na b B T args S} : 
+  wf Σ.1 ->
+  typing_spine Σ Γ (T {0 := b}) args S ->
+  isWfArity_or_Type Σ Γ (tProd na B T) ->
+  Σ ;;; Γ |- b : B ->
+  typing_spine Σ Γ (tProd na B T) (b :: args) S.
+Proof.
+  intros wfΣ Hsp.
+  depelim Hsp.
+  econstructor; eauto. constructor; auto.
+  intros Har. eapply isWAT_tProd in Har as [? ?]; eauto using typing_wf_local.
+  intros Hb.
+  econstructor. 3:eauto. 2:eauto. 
+  destruct i1 as [[ctx [s [Hs ?]]]|?].
+  - left. exists ([vass na B] ,,, ctx), s; simpl; intuition auto.
+    rewrite destArity_app Hs /= ?app_context_nil_l //.
+    now rewrite app_context_assoc.
+  - right. destruct i1 as [s Hs], i0 as [s' Hs'].
+    eexists. eapply type_Prod; eauto.
+  - econstructor; eauto.
+Qed.
+
+Lemma typing_spine_WAT_concl {cf:checker_flags} {Σ Γ T args S} : 
+  typing_spine Σ Γ T args S ->
+  isWfArity_or_Type Σ Γ S.
+Proof.
+  induction 1; auto.
+Qed.
+
+Lemma isWAT_wf_local {cf:checker_flags} {Σ Γ T} : isWfArity_or_Type Σ Γ T -> wf_local Σ Γ.
+Proof.
+  move=> [[ctx [s [_ Hs]]]|[s Hs]]. 
+  - eapply All_local_env_app in Hs.
+    intuition eauto with pcuic.
+  - now eapply typing_wf_local.
+Qed.  
+
+
+(** This lemmma is complicated by the fact that `args` might be an instance
+    of arguments for a convertible arity of `ind`.
+    Actually #|args| must be exactly of the length of the number of parameters
+    + indices (lets excluded). *)
+    Lemma inversion_WAT_indapp {cf:checker_flags} Σ Γ ind u args :
+    forall mdecl idecl (isdecl : declared_inductive Σ.1 mdecl ind idecl),
+    wf Σ.1 ->
+    isType Σ Γ (mkApps (tInd ind u) args) ->
+    mdecl.(ind_npars) <= #|args| /\ inductive_ind ind < #|ind_bodies mdecl| /\
+    consistent_instance_ext Σ (ind_universes mdecl) u.
+Proof.
+  intros mdecl idecl decli wfΣ cty.
+  destruct cty as [s Hs].
+  pose proof (typing_wf_local Hs).
+  eapply type_mkApps_inv in Hs as [T' [U' [[H Hspine] H']]]; auto.
+  have validT' := (validity _ _ _ _ _ _ H).
+  specialize (validT' wfΣ (typing_wf_local H)).
+  destruct validT' as [_ validT'].
+  eapply inversion_Ind in H as [mdecl' [idecl' [wfl [decli' [univs ?]]]]]; auto.
+  destruct decli, decli'.
+  red in H, H1. rewrite H in H1. noconf H1.
+  rewrite H0 in H2. noconf H2.
+  assert (declared_inductive Σ.1 mdecl ind idecl).
+  split; auto.
+  apply on_declared_inductive in H1 as [onmind onind]; auto.
+  rewrite (ind_arity_eq onind) in c; auto.
+  rewrite !subst_instance_constr_it_mkProd_or_LetIn in c.
+  simpl in c.
+  eapply invert_cumul_arity_l in c; auto.
+  rewrite !destArity_it_mkProd_or_LetIn in c.
+  destruct c as [T'0 [ctx' [s' [[[redT' destT'] convctx]leq]]]].
+  eapply isWfArity_or_Type_red in validT'. 3:eapply redT'. 2:auto.
+  eapply typing_spine_strengthen in Hspine; last first.
+  eapply red_cumul_inv, redT'. all:eauto.
+  generalize (destArity_spec [] T'0). rewrite destT'.
+  simpl; intros ->.
+  pose proof (context_relation_length _ _ _ convctx).
+  assert(assumption_context ctx').
+  { eapply context_relation_app in convctx as [convΓ convctx'].
+    eapply conv_context_smash in convctx'.
+    auto. eapply smash_context_assumption_context. constructor.
+    rewrite smash_context_length. simpl.
+    rewrite !app_context_length smash_context_length /= in H1.
+    lia.
+  }
+  assert(wf_local Σ (Γ ,,, ctx')).
+  { destruct validT'.
+    destruct i as [ctx'' [s'' [i j]]].
+    rewrite destArity_it_mkProd_or_LetIn /= in i. noconf i. 
+    rewrite app_context_nil_l in j. apply j.
+    destruct i as [i Hs].
+    eapply inversion_it_mkProd_or_LetIn in Hs.
+    eauto using typing_wf_local. auto. auto. }
+  destruct Hspine as [U'concl [sp' cum']].
+  rewrite app_context_length smash_context_length /= app_context_nil_l context_assumptions_app in H1.
+  rewrite !subst_instance_context_assumptions onmind.(onNpars _ _ _ _) app_context_length in H1.
+  clear destT' redT'.
+  eapply typing_spine_weaken_concl in sp'.
+  3:{ transitivity U'. eapply cum'. eapply H'. }
+  eapply arity_typing_spine in sp'; eauto.
+  destruct sp'.
+  rewrite H3 (assumption_context_length ctx') //.
+  split. lia. now eapply nth_error_Some_length in H0.
+  auto.
+  left. eexists _, _; intuition auto.
+Qed.
