pcuic/theories/PCUICConfluence.v
@@ -1050,19 +1050,6 @@ Proof.
     rewrite !app_context_assoc. cbn. intuition.
 Qed.
 
-Lemma mapi_rec_compose {A B C} (g : nat -> B -> C) (f : nat -> A -> B) k l :
-  mapi_rec g (mapi_rec f l k) k = mapi_rec (fun k x => g k (f k x)) l k.
-Proof.
-  induction l in k |- *; simpl; auto. now rewrite IHl.
-Qed.
-
-Lemma mapi_compose {A B C} (g : nat -> B -> C) (f : nat -> A -> B) l :
-  mapi g (mapi f l) = mapi (fun k x => g k (f k x)) l.
-Proof. apply mapi_rec_compose. Qed.
-
-Lemma mapi_cst_map {A B} (f : A -> B) l : mapi (fun _ => f) l = map f l.
-Proof. unfold mapi. generalize 0. induction l; cbn; auto. intros. now rewrite IHl. Qed.
-
 Lemma All_All2_telescopei_gen P (Γ Γ' Δ Δ' : context) (m m' : mfixpoint term) :
   (forall Δ Δ' x y,
     All2_local_env_over P Γ Γ' Δ Δ' ->
