pcuic/theories/PCUICCtxShape.v
@@ -1,0 +1,64 @@
+Definition same_shape (d d' : context_decl) := 
+  match decl_body d, decl_body d' with
+  | None, None => True
+  | Some _, Some _ => True
+  | _, _ => False
+  end.
+  
+Definition same_ctx_shape (Γ Γ' : context) :=
+  context_relation (fun _ _ => same_shape) Γ Γ'.
+  
+Hint Unfold same_ctx_shape : core.
+
+Lemma same_ctx_shape_app Γ Γ' Δ Δ' : same_ctx_shape Γ Γ' -> 
+  same_ctx_shape Δ Δ' ->
+  same_ctx_shape (Γ ++ Δ)%list (Γ' ++ Δ')%list.
+Proof.
+  induction 1; simpl; try constructor; auto. 
+  apply IHcontext_relation. auto.
+  apply IHcontext_relation. auto.
+Qed.
+
+Lemma same_ctx_shape_rev Γ Γ' : same_ctx_shape Γ Γ' -> 
+  same_ctx_shape (List.rev Γ) (List.rev Γ').
+Proof.
+  induction 1; simpl; try constructor.
+  apply same_ctx_shape_app; auto. repeat constructor.
+  apply same_ctx_shape_app; auto. repeat constructor.
+Qed.
+
+Lemma context_assumptions_app Γ Γ' : context_assumptions (Γ ++ Γ')%list = 
+  context_assumptions Γ + context_assumptions Γ'.
+Proof.
+  induction Γ; simpl; auto.
+  destruct a as [? [?|] ?]; simpl; auto.
+Qed.
+
+Lemma instantiate_params_ok ctx ctx' pars t : 
+  same_ctx_shape ctx ctx' -> #|pars| = context_assumptions ctx ->
+  ∑ h, instantiate_params ctx pars (it_mkProd_or_LetIn ctx' t) = Some h.
+Proof.
+  intros Hctx Hpars. rewrite instantiate_params_.
+  apply same_ctx_shape_rev in Hctx.
+  rewrite -(List.rev_involutive ctx').
+  rewrite -(List.rev_involutive ctx) in Hpars.
+  generalize (@nil term).
+  induction Hctx in t, pars, Hpars |- *.
+  - simpl. destruct pars; try discriminate. simpl in Hpars. intros l.
+    now eexists (subst0 l _).
+  - destruct pars; try discriminate.
+    simpl in Hpars. rewrite context_assumptions_app in Hpars.
+    simpl in Hpars. elimtype False. omega.
+    simpl in Hpars. rewrite context_assumptions_app in Hpars.
+    rewrite Nat.add_1_r in Hpars. noconf Hpars.
+    simpl in H.
+    intros l.
+    destruct (IHHctx _ t H (t0 :: l)).
+    simpl. exists x.
+    now rewrite it_mkProd_or_LetIn_app.
+  - intros l.
+    simpl in Hpars. rewrite context_assumptions_app in Hpars.
+    simpl in Hpars. rewrite Nat.add_0_r in Hpars. simpl.
+    rewrite it_mkProd_or_LetIn_app.
+    simpl. apply IHHctx. auto.
+Qed.
